pulse/lib/steel/pulse/Pulse.Soundness.WithLocal.fst
@@ -1,0 +1,16 @@
+module Pulse.Soundness.WithLocal
+
+open Pulse.Syntax
+open Pulse.Reflection.Util
+open Pulse.Typing
+open Pulse.Elaborate.Pure
+open Pulse.Elaborate.Core
+open Pulse.Elaborate
+open Pulse.Soundness.Common
+
+module R = FStar.Reflection
+
+module PReflUtil = Pulse.Reflection.Util
+module WT = Pulse.Steel.Wrapper.Typing
+
+let withlocal_soundness #f #g #t #c d soundness = admit ()
